Source/IntegrationTests/TestFiles/LitTests/LitTest/concurrency-sound/concurrency-test2.dfy
@@ -1,0 +1,10 @@
+trait Holder<T> {
+  var value: T
+}
+
+method {:concurrent} Test(holder: Holder<int>)
+{
+  var x := holder.value + holder.value;
+  assert holder.value + holder.value == 2*holder.value;
+  assert x == holder.value + holder.value;
+}
